theories/LRInduction.v
@@ -5,7 +5,7 @@ Section Inductions.
   Context `{ta : tag}
     `{!WfContext ta} `{!WfType ta} `{!Typing ta}
     `{!ConvType ta} `{!ConvTerm ta} `{!ConvNeu ta}
-    `{!OneRedType ta} `{!OneRedTerm ta}.
+    `{!RedType ta} `{!RedTerm ta}.
 
   #[universes(polymorphic)]Fixpoint LR_embedding {l l'} (l_ : l << l')
     {Γ A rEq rTe rTeEq} (lr : LogRel l Γ A rEq rTe rTeEq) {struct lr} : (LogRel l' Γ A rEq rTe rTeEq) :=
