theories/Reduction.v
@@ -1,5 +1,6 @@
+From Coq Require Import CRelationClasses.
 From LogRel.AutoSubst Require Import core unscoped Ast.
-From LogRel Require Import Utils BasicAst Notations Context Untyped Weakening GenericTyping DeclarativeTyping Generation.
+From LogRel Require Import Utils BasicAst Notations Context Untyped UntypedReduction Weakening GenericTyping DeclarativeTyping Generation.
 
 Import DeclarativeTypingData.
 
@@ -20,9 +21,9 @@ Definition RedConvTeC {Γ} {t u A : term} :
     [Γ |- t ≅ u : A].
 Proof.
   induction 1.
-  1: now constructor.
-  eapply TermTrans ; tea.
-  now apply RedConvTe.
+  - now constructor.
+  - now eapply RedConvTe.
+  - now eapply TermTrans.
 Qed.
 
 Definition RedConvTy {Γ} {A B : term} :
@@ -30,7 +31,7 @@ Definition RedConvTy {Γ} {A B : term} :
     [Γ |- A ≅ B].
 Proof.
   destruct 1.
-  now (econstructor ; eapply RedConvTe ; eassumption).
+  now econstructor ; eapply RedConvTe.
 Qed.
 
 Definition RedConvTyC {Γ} {A B : term} :
@@ -38,9 +39,9 @@ Definition RedConvTyC {Γ} {A B : term} :
     [Γ |- A ≅ B].
 Proof.
   induction 1.
-  1: now econstructor.
-  eapply TypeTrans ; tea.
-  now apply RedConvTy.
+  - now constructor.
+  - now eapply RedConvTy.
+  - now eapply TypeTrans.
 Qed.
 
 Lemma InfRedTy {Γ A t} :
@@ -52,87 +53,24 @@ Proof.
   now apply RedConvTyC.
 Qed.
 
-(** Whnf do not reduce *)
-
-Lemma whne_nored Γ n u A :
-  whne Γ n -> [Γ |- n ⇒ u : A] -> False.
+Lemma oredtm_meta_conv (Γ : context) (t u u' A A' : term) :
+  [Γ |- t ⇒ u : A] ->
+  A' = A ->
+  u' = u ->
+  [Γ |- t ⇒ u' : A'].
 Proof.
-  intros ne red.
-  induction red in ne |- * ; fold_decl.
-  - inversion ne ; subst ; clear ne.
-    eapply neLambda.
-    eassumption.
-  - inversion ne ; subst.
-    1: easy.
-  - easy.
+  now intros ? -> ->.
 Qed.
 
-Lemma whnf_nored Γ n u A :
-  whnf Γ n -> [Γ |- n ⇒ u : A] -> False.
-Proof.
-  intros nf red.
-  induction red in nf |- *.
-  - inversion nf ; subst.
-    inversion H ; subst.
-    eapply neLambda.
-    eassumption.
-  - inversion nf ; subst.
-    inversion H ; subst.
-    eapply IHred.
-    now constructor.
-  - easy.
-Qed.
+(* Weakenings *)
 
-Corollary whnf_nored_ty Γ A B : [Γ |- A ⇒ B] -> whnf Γ A -> False.
-Proof.
-  intros [].
-  eauto using whnf_nored.
-Qed.
-
-
-(** Determinism of reduction *)
-
-Lemma red_det {Γ t u v A B} :
-  [Γ |- t ⇒ u : A] -> [Γ |- t ⇒ v : B] ->
-  u = v.
-Proof.
-  intros red red'.
-  induction red in v, B, red' |- *.
-  - eapply termRedGen in red' as [? [d]].
-    inversion d ; subst ; clear d.
-    + exfalso.
-      eapply whnf_nored.
-      2: eassumption.
-      now econstructor.
-    + reflexivity.
-  - eapply termRedGen in red' as [? [d]].
-    inversion d ; subst ; clear d.
-    + f_equal.
-      eauto.
-    + exfalso.
-      eapply whnf_nored.
-      2: eassumption.
-      now econstructor.
-  - easy.
-Qed.
-
-Lemma red_det_ty {Γ A B C} :
-  [Γ |- A ⇒ B] -> [Γ |- A ⇒ C] ->
-  B = C.
-Proof.
-  intros HB HB'.
-  destruct HB, HB'.
-  now eapply red_det.
-Qed.
-
-
-Lemma redtm_wk {Γ Δ t u A} (ρ : Δ ≤ Γ) :
+Lemma oredtmdecl_wk {Γ Δ t u A} (ρ : Δ ≤ Γ) :
 [|- Δ ] -> [Γ |- t ⇒ u : A] -> [Δ |- t⟨ρ⟩ ⇒ u⟨ρ⟩ : A⟨ρ⟩].
 Proof.
   intros ? red.
   induction red as [? ? ? ? ? ? Ht Ha | |]; fold_decl.
   - cbn in *.
-    eapply redtm_meta_conv.
+    eapply oredtm_meta_conv.
     1: econstructor ; fold_decl.
     1,3: now eapply typing_wk.
     + unshelve eapply typing_wk in Ht.
@@ -140,14 +78,13 @@ Proof.
       1: shelve.
       2: now econstructor ; [eassumption | eapply typing_wk].
       cbn in *.
-      now replace (ren_term _ t) with (t⟨wk_up ρ⟩)
-        by (cbn ; now asimpl).
+      now apply Ht.
     + unfold ren1, RenWlWk_term.
       cbn.
       now asimpl.
     + now asimpl. 
   - cbn in *.
-    eapply redtm_meta_conv.
+    eapply oredtm_meta_conv.
     1: econstructor ; fold_decl.
     + now eauto.
     + now eapply typing_wk.
@@ -158,15 +95,125 @@ Proof.
     now eapply typing_wk.
 Qed.
 
-Lemma redty_wk {Γ Δ A B} (ρ : Δ ≤ Γ) :
-[|- Δ ] -> [Γ |- A ⇒ B] -> [Δ |- A⟨ρ⟩ ⇒ B⟨ρ⟩].
+Lemma redtmdecl_wk {Γ Δ t u A} (ρ : Δ ≤ Γ) :
+  [|- Δ ] -> [Γ |- t ⇒* u : A] -> [Δ |- t⟨ρ⟩ ⇒* u⟨ρ⟩ : A⟨ρ⟩].
+Proof.
+  intros * ?.
+  induction 1.
+  - econstructor ; now apply typing_wk.
+  - econstructor ; now eapply oredtmdecl_wk.
+  - now econstructor.
+Qed.
+
+Lemma oredtydecl_wk {Γ Δ A B} (ρ : Δ ≤ Γ) :
+  [|- Δ ] -> [Γ |- A ⇒ B] -> [Δ |- A⟨ρ⟩ ⇒ B⟨ρ⟩].
 Proof.
   intros ? red.
   destruct red.
   constructor.
   fold_decl.
   change U with (U⟨ρ⟩).
-  now apply redtm_wk.
+  now apply oredtmdecl_wk.
+Qed.
+
+Lemma redtydecl_wk {Γ Δ A B} (ρ : Δ ≤ Γ) :
+  [|- Δ ] -> [Γ |- A ⇒* B] -> [Δ |- A⟨ρ⟩ ⇒* B⟨ρ⟩].
+Proof.
+  intros * ?.
+  induction 1.
+  - now econstructor ; apply typing_wk.
+  - now econstructor ; eapply oredtydecl_wk.
+  - now econstructor.
+Qed.
+
+(* Type erasure *)
+
+Lemma oredtmdecl_ored Γ t u A : 
+  [Γ |- t ⇒ u : A] ->
+  [t ⇒ u].
+Proof.
+  induction 1.
+  1-2: now econstructor.
+  eassumption.
+Qed.
+
+Lemma redtmdecl_red Γ t u A : 
+  [Γ |- t ⇒* u : A] ->
+  [t ⇒* u].
+Proof.
+  induction 1.
+  - now econstructor.
+  - econstructor ; eauto using oredtmdecl_ored.
+    reflexivity.
+  - now etransitivity.
+Qed.
+
+Lemma oredtydecl_ored Γ A B : 
+  [Γ |- A ⇒ B] ->
+  [A ⇒ B].
+Proof.
+  induction 1.
+  now eapply oredtmdecl_ored.
+Qed.
+
+Lemma redtydecl_red Γ A B : 
+  [Γ |- A ⇒* B] ->
+  [A ⇒* B].
+Proof.
+  induction 1.
+  - now econstructor.
+  - econstructor ; eauto using oredtydecl_ored.
+    reflexivity.
+  - now etransitivity.
+Qed.
+
+(* Lifting rules from ⇒ to ⇒* *)
+
+Lemma redtmdecl_app Γ na A B f f' t :
+  [ Γ |- f ⇒* f' : tProd na A B ] ->
+  [ Γ |- t : A ] ->
+  [ Γ |- tApp f t ⇒* tApp f' t : B[t..] ].
+Proof.
+  intros Hf ?.
+  remember (tProd na A B) as T in *.
+  induction Hf.
+  + subst.
+    now do 2 econstructor.
+  + subst.
+    now do 2 econstructor.
+  + now econstructor.
+Qed.
+
+Lemma redtmdecl_conv Γ t u A A' : 
+  [Γ |- t ⇒* u : A] ->
+  [Γ |- A ≅ A'] ->
+  [Γ |- t ⇒* u : A'].
+Proof.
+  intros Ht ?.
+  induction Ht.
+  + now do 2 econstructor.
+  + now do 2 econstructor.
+  + now econstructor.
+Qed.
+
+Lemma redtydecl_term Γ A B :
+  [ Γ |- A ⇒* B : U] -> [Γ |- A ⇒* B ].
+Proof.
+  remember U as T.
+  induction 1 ; subst.
+  + now do 2 econstructor.
+  + now do 2 econstructor.
+  + now econstructor.
+Qed.
+
+#[export] Instance RedTermTrans Γ A : Transitive (red_tm Γ A).
+Proof.
+  now econstructor.
+Qed.
+
+#[export] Instance RedTypeTrans Γ : Transitive (red_ty Γ).
+Proof.
+  now econstructor.
 Qed.
 
 Module DeclarativeTypingProperties.
@@ -181,8 +228,8 @@ Module DeclarativeTypingProperties.
     - now eapply WFterm. 
     - now eapply WFEqType.
     - now eapply WFEqTerm.
-    - now eapply WFEqType, RedConvTy.
-    - now eapply WFEqTerm, RedConvTe. 
+    - now eapply WFEqType, RedConvTyC.
+    - now eapply WFEqTerm, RedConvTeC. 
   Qed.
 
   #[export, refine] Instance WfTypeProperties : WfTypeProperties (ta := de) := {}.
@@ -271,30 +318,30 @@ Module DeclarativeTypingProperties.
     now econstructor.
   Qed.
   
-  #[export, refine] Instance OneRedTermDeclProperties : OneRedTermProperties (ta := de) := {}.
+  #[export, refine] Instance RedTermDeclProperties : RedTermProperties (ta := de) := {}.
   Proof.
   - intros.
-    now eapply redtm_wk.
+    now eapply redtmdecl_wk.
   - intros.
-    eapply whnf_nored ; eassumption.
+    now eapply redtmdecl_red.
   - intros.
-    now eapply red_det.
+    now do 2 econstructor.
   - intros.
-    now econstructor.
+    now eapply redtmdecl_app.
   - intros.
-    now econstructor.
+    now eapply redtmdecl_conv.
   - intros.
     now econstructor.
   Qed. 
 
-  #[export, refine] Instance OneRedTypeDeclProperties : OneRedTypeProperties (ta := de) := {}.
+  #[export, refine] Instance RedTypeDeclProperties : RedTypeProperties (ta := de) := {}.
   Proof.
   - intros.
-    now eapply redty_wk.
+    now eapply redtydecl_wk.
   - intros.
-    now eapply whnf_nored_ty.
+    now eapply redtydecl_red.
   - intros.
-    now eapply red_det_ty.
+    now eapply redtydecl_term.
   - intros.
     now econstructor.
   Qed.
